feat: soundness of normalizeAux

Lean4Lean/Verify/Level.lean
@@ -2,8 +2,90 @@ import Lean4Lean.Theory.VLevel
 import Lean4Lean.Level
 import Lean4Lean.Verify.Axioms
 import Std.Tactic.BVDecide
+import Std.Data.TreeMap.Lemmas
 
-namespace Lean.Level
+namespace Lean
+
+namespace Name
+open Std
+
+instance : TransCmp cmp := by
+  have eq_swap {a b : Name} : a.cmp b = (b.cmp a).swap := by
+    induction a generalizing b with obtain _|⟨b₁,b₂⟩|⟨b₁,b₂⟩ := b <;> simp [cmp]
+    | str a₁ a₂ ih | num a₁ a₂ ih =>
+      rw [ih]; cases b₁.cmp a₁ <;> simp [← OrientedOrd.eq_swap]
+  refine { eq_swap, isLE_trans {a b c} := ?_ }
+  have {α} [Ord α] [TransOrd α] {a₁ b₁ c₁} {a₂ b₂ c₂ : α}
+      (H1 : (cmp a₁ b₁).isLE → (cmp b₁ c₁).isLE → (cmp a₁ c₁).isLE)
+      (H2 : (cmp c₁ a₁).isLE → (cmp a₁ b₁).isLE → (cmp c₁ b₁).isLE)
+      (H3 : (cmp b₁ c₁).isLE → (cmp c₁ a₁).isLE → (cmp b₁ a₁).isLE) :
+      ((cmp a₁ b₁).then (compare a₂ b₂)).isLE →
+      ((cmp b₁ c₁).then (compare b₂ c₂)).isLE →
+      ((cmp a₁ c₁).then (compare a₂ c₂)).isLE := by
+    simp [Ordering.isLE_then_iff_and]
+    intro h1 h2 h3 h4
+    refine have := H1 h1 h3; ⟨this, ?_⟩
+    obtain eq | eq := Ordering.isLE_iff_eq_lt_or_eq_eq.1 this; · exact .inl eq
+    obtain h2 | h2 := h2
+    · rw [@eq_swap c₁, eq, @eq_swap _ a₁, h2] at H3; simp [h3] at H3
+    obtain h4 | h4 := h4
+    · rw [eq_swap, eq, @eq_swap c₁, h4] at H2; simp [h1] at H2
+    exact .inr (TransCmp.isLE_trans h2 h4)
+  refine (?_ : _ ∧ ((cmp c a).isLE → (cmp a b).isLE → (cmp c b).isLE) ∧
+    ((cmp b c).isLE → (cmp c a).isLE → (cmp b a).isLE)).1
+  induction a generalizing b c with
+    obtain _|⟨b₁,b₂⟩|⟨b₁,b₂⟩ := b <;> simp [cmp] at * <;>
+    obtain _|⟨c₁,c₂⟩|⟨c₁,c₂⟩ := c <;> simp [cmp] at *
+  | str a₁ a₂ ih | num a₁ a₂ ih =>
+    let ⟨h1, h2, h3⟩ := @ih b₁ c₁
+    exact ⟨this h1 h2 h3, this h2 h3 h1, this h3 h1 h2⟩
+
+instance : LawfulBEqCmp cmp where
+  compare_eq_iff_beq {a b} := by
+    simp; refine ⟨?_, fun h => h ▸ ReflCmp.compare_self⟩
+    induction a generalizing b with obtain _|⟨b₁,b₂⟩|⟨b₁,b₂⟩ := b <;> simp [cmp]
+    | str a₁ a₂ ih | num a₁ a₂ ih =>
+      refine ?_ ∘ Ordering.then_eq_eq.1
+      simp +contextual; exact fun h _ => ih h
+
+instance : TransCmp quickCmp where
+  eq_swap {a b} := by
+    simp [quickCmp]
+    rw [OrientedOrd.eq_swap]
+    cases compare b.hash a.hash <;> simp
+    induction a generalizing b with obtain _|⟨b₁,b₂⟩|⟨b₁,b₂⟩ := b <;> simp [quickCmpAux]
+    | str a₁ a₂ ih | num a₁ a₂ ih =>
+      rw [OrientedOrd.eq_swap]
+      cases compare b₂ a₂ <;> simp [ih]
+  isLE_trans {a b c} := by
+    have {α} [Ord α] [TransOrd α] {a₁ b₁ c₁ : α} {a₂ b₂ c₂}
+        (H : (quickCmpAux a₂ b₂).isLE → (quickCmpAux b₂ c₂).isLE → (quickCmpAux a₂ c₂).isLE) :
+        ((compare a₁ b₁).then (quickCmpAux a₂ b₂)).isLE →
+        ((compare b₁ c₁).then (quickCmpAux b₂ c₂)).isLE →
+        ((compare a₁ c₁).then (quickCmpAux a₂ c₂)).isLE := by
+      simp [Ordering.isLE_then_iff_and]
+      intro h1 h2 h3 h4
+      refine ⟨TransCmp.isLE_trans h1 h3, ?_⟩
+      refine h2.elim (fun h2 => .inl <| TransCmp.lt_of_lt_of_isLE h2 h3) fun h2 => ?_
+      refine h4.elim (fun h4 => .inl <| TransCmp.lt_of_isLE_of_lt h1 h4) fun h4 => .inr (H h2 h4)
+    apply this
+    induction a generalizing b c with
+      obtain _|⟨b₁,b₂⟩|⟨b₁,b₂⟩ := b <;> simp [quickCmpAux] at * <;>
+      obtain _|⟨c₁,c₂⟩|⟨c₁,c₂⟩ := c <;> simp [quickCmpAux] at *
+    | str a₁ a₂ ih | num a₁ a₂ ih => apply this ih
+
+instance : LawfulBEqCmp quickCmp where
+  compare_eq_iff_beq {a b} := by
+    simp; refine ⟨fun h => ?_, fun h => h ▸ ReflCmp.compare_self⟩
+    replace h := (Ordering.then_eq_eq.1 h).2; revert h
+    induction a generalizing b with obtain _|⟨b₁,b₂⟩|⟨b₁,b₂⟩ := b <;> simp [quickCmpAux]
+    | str a₁ a₂ ih | num a₁ a₂ ih =>
+      refine ?_ ∘ Ordering.then_eq_eq.1
+      simp +contextual; exact fun _ => ih
+
+end Name
+
+namespace Level
 open Lean4Lean
 
 attribute [simp] mkLevelSucc mkLevelMax mkLevelIMax updateSucc! updateMax! updateIMax!
@@ -154,8 +236,352 @@ open private substParams.go from Lean.Level in
 theorem substParams_id {u : Level} :
     substParams' .param false u = u := by induction u <;> simp_all [substParams']
 
+local notation "max'" => Max.max
+
+namespace Normalize
+
+attribute [local instance] Lean.Level.Normalize.instOrdName_lean4Lean
+
+local instance : Std.TransCmp (α := Name) compare := inferInstanceAs (Std.TransCmp Name.cmp)
+local instance : Std.LawfulBEqCmp (α := List Name) compare :=
+  inferInstanceAs (Std.LawfulBEqCmp (List.compareLex Name.cmp))
+
+instance : LawfulBEq VarNode where
+  rfl {a} := by cases a <;> simp! [instBEqVarNode]
+  eq_of_beq {a b} := by cases a <;> cases b <;> simp! [instBEqVarNode]
+
+@[reducible] local instance : Membership (List Name) NormLevel :=
+  inferInstanceAs (Membership _ (Std.TreeMap _ _ compare))
+
+@[reducible] local instance : GetElem? NormLevel (List Name) Node (fun m a => a ∈ m) :=
+  inferInstanceAs (GetElem? (Std.TreeMap _ _ compare) ..)
+
+section
+variable (ls : List Name) (ρ : List Nat) in
+def evalParam (x : Name) : Nat :=
+let i := ls.idxOf x; if i < ls.length then ρ[i]?.getD 0 else 0
+
+theorem evalParam_eq (hv : ls.idxOf x < ls.length) :
+    evalParam ls ρ x = ρ[List.idxOf x ls]?.getD 0 := if_pos hv
+
+variable (ls : List Name) (ρ : List Nat) in
+def VarNode.eval (l : VarNode) : Nat := evalParam ls ρ l.var + l.offset
+
+variable (ls : List Name) (ρ : List Nat) in
+def Node.eval (l : Node) : Nat :=
+  l.var.foldl (init := l.const) fun n v => max' n (v.eval ls ρ)
+
+theorem Node.eval_le : eval ls ρ l ≤ n ↔
+    l.const ≤ n ∧ ∀ v ∈ l.var, v.eval ls ρ ≤ n := by
+  simp [eval, ← List.foldr_reverse]; simp only [← l.var.mem_reverse]
+  induction l.var.reverse with simp | cons a l
+  simp [Nat.max_le, and_comm, and_left_comm, *]
+
+variable (ls : List Name) (ρ : List Nat) in
+def allNZ (path : List Name) : Bool := path.all (0 < evalParam ls ρ ·)
+
+theorem allNZ_cons : allNZ ls ρ (a :: path) ↔
+    0 < evalParam ls ρ a ∧ allNZ ls ρ path := by simp [allNZ]
+
+theorem allNZ_mono (H : ∀ x ∈ path, x ∈ path') : allNZ ls ρ path' → allNZ ls ρ path := by
+  simp [allNZ]; grind
+
+variable (ls : List Name) (ρ : List Nat) in
+def evalPath (path : List Name) (n : Nat) : Nat :=
+  if allNZ ls ρ path then n else 0
+
+theorem evalPath_cons : evalPath ls ρ (a :: path) n =
+    evalPath ls ρ path (if 0 < evalParam ls ρ a then n else 0) := by
+  by_cases h : 0 < evalParam ls ρ a <;> simp [evalPath, allNZ_cons, h]
+
+theorem evalPath_max :
+    evalPath ls ρ path (max' m n) = max' (evalPath ls ρ path m) (evalPath ls ρ path n) := by
+  simp [evalPath]; split <;> simp
+
+theorem evalPath_mono (h : n ≤ m) :
+    evalPath ls ρ path n ≤ evalPath ls ρ path m := by
+  simp [evalPath]; split <;> simp [*]
+
+theorem evalPath_le : evalPath ls ρ path n ≤ m ↔ (allNZ ls ρ path → n ≤ m) := by
+  simp [evalPath]; split <;> simp [*]
+
+variable (ls : List Name) (ρ : List Nat) in
+inductive EvalPaths : List Name → Nat → Prop
+  | nil : EvalPaths [] n
+  | insert : orderedInsert Name.cmp a path = some path' →
+    evalPath ls ρ path (evalParam ls ρ a) ≤ n → EvalPaths path n → EvalPaths path' n
+
+theorem EvalPaths.mono (h : n ≤ n') : EvalPaths ls ρ path n → EvalPaths ls ρ path n'
+  | .nil => .nil
+  | .insert h1 h2 h3 => .insert h1 (Nat.le_trans h2 h) (h3.mono h)
+
+theorem EvalPaths.max : EvalPaths ls ρ path n → EvalPaths ls ρ path (max' n m) :=
+  .mono (Nat.le_max_left ..)
+
+variable (ls : List Name) (ρ : List Nat) in
+def NormLevel.eval (l : NormLevel) : Nat :=
+  l.foldl (init := 0) fun n a b => max' n (evalPath ls ρ a (b.eval ls ρ))
+
+theorem NormLevel.eval_le : eval ls ρ l ≤ n ↔
+    ∀ a b, l.get? a = some b → evalPath ls ρ a (b.eval ls ρ) ≤ n := by
+  simp [eval, Std.TreeMap.foldl_eq_foldl_toList, ← List.foldr_reverse]
+  simp only [← Std.TreeMap.mem_toList_iff_getElem?_eq_some, ← l.toList.mem_reverse]
+  induction l.toList.reverse with simp | cons a l; let (a, b) := a
+  simp [or_imp, forall_and, Nat.max_le, and_comm, *]
+
+end
+
+theorem NormLevel.addVar_contains (H : acc.contains x) : (addVar v k path acc).contains x := by
+  simp_all [addVar, Std.TreeMap.mem_modify]
+
+theorem NormLevel.addNode_contains (H : acc.contains x) : (addNode v k path acc).contains x := by
+  simp [addNode, Std.TreeMap.mem_alter] at *; split <;> simp [*]
+
+theorem NormLevel.addNode_contains_self : (addNode v k path acc).contains path := by
+  simp [addNode]; split <;> simp
+
+theorem NormLevel.addConst_contains (H : acc.contains x) : (addConst k path acc).contains x := by
+  simp [addConst] at *; split <;> simp [H, Std.TreeMap.mem_modify]
+
+theorem normalizeAux_contains (H : acc.contains x) : (normalizeAux u path k acc).contains x := by
+  unfold normalizeAux; split
+  · exact NormLevel.addConst_contains H
+  · exact NormLevel.addConst_contains H
+  · exact normalizeAux_contains H
+  · exact normalizeAux_contains (normalizeAux_contains H)
+  · exact normalizeAux_contains (normalizeAux_contains H)
+  · exact normalizeAux_contains (normalizeAux_contains H)
+  · exact normalizeAux_contains (normalizeAux_contains H)
+  · split <;> [skip; (dsimp; split)]
+    · exact normalizeAux_contains (NormLevel.addNode_contains (NormLevel.addConst_contains H))
+    · exact normalizeAux_contains H
+    · exact normalizeAux_contains (NormLevel.addVar_contains H)
+  · exact H
+  · exact H
+  · split <;> [skip; split]
+    · exact NormLevel.addNode_contains (NormLevel.addConst_contains H)
+    · exact H
+    · exact NormLevel.addVar_contains H
+
+theorem imax_max : Nat.imax a (max' b c) = max' (Nat.imax a b) (Nat.imax a c) := by
+  simp [Nat.imax]; symm; split <;> simp [*]; split <;> simp [*, Nat.max_eq_max]
+  rw [Nat.max_left_comm b, ← Nat.max_assoc, Nat.max_self]
+
+theorem imax_imax : Nat.imax a (Nat.imax b c) = max' (Nat.imax a c) (Nat.imax b c) := by
+  simp [Nat.imax]; by_cases h : c = 0 <;> simp [*, Nat.max_eq_max]
+  rw [Nat.max_left_comm c, Nat.max_self]
+
+theorem mem_orderedInsert [BEq α] [LawfulBEq α] [Std.LawfulBEqCmp (α := α) cmp] :
+    b ∈ (orderedInsert cmp a ls).getD ls ↔ b = a ∨ b ∈ ls := by
+  induction ls <;> simp [orderedInsert]; split <;> simp_all [or_left_comm]
+
+theorem allNZ_orderedInsert :
+    allNZ ls ρ ((orderedInsert Name.cmp a path).getD path) = allNZ ls ρ (a :: path) := by
+  rw [Bool.eq_iff_iff]; simp [allNZ, mem_orderedInsert]
+
+theorem evalPath_orderedInsert :
+    evalPath ls ρ ((orderedInsert Name.cmp a path).getD path) = evalPath ls ρ (a :: path) := by
+  ext n; simp [evalPath, allNZ_orderedInsert]
+
+theorem EvalPaths.of_mem (hm : v ∈ path) (H : EvalPaths ls ρ path n) :
+    ∃ path₁ path₂, (∀ x ∈ path₁, x ∈ path) ∧
+      orderedInsert Name.cmp v path₁ = some path₂ ∧
+      evalPath ls ρ path₁ (evalParam ls ρ v) ≤ n ∧
+      EvalPaths ls ρ path₁ n := by
+  induction H with | nil => cases hm | insert h1 h2 h3 ih
+  obtain rfl | hm := (h1 ▸ mem_orderedInsert).1 hm
+  · exact ⟨_, _, fun _ h => (h1 ▸ mem_orderedInsert).2 (.inr h), h1, h2, h3⟩
+  · let ⟨_, _, a1, a2, a3, a4⟩ := ih hm
+    exact ⟨_, _, fun _ h => (h1 ▸ mem_orderedInsert).2 (.inr (a1 _ h)), a2, a3, a4⟩
+
+theorem ext_le {n m : Nat} (H : ∀ x, n ≤ x ↔ m ≤ x) : n = m :=
+  Nat.le_antisymm ((H _).2 (Nat.le_refl _)) ((H _).1 (Nat.le_refl _))
+
+theorem le_ext_le {n m : Nat} (H : ∀ x, n ≤ x → m ≤ x) : m ≤ n := H _ (Nat.le_refl _)
+
+theorem NormLevel.addConst_eval
+    (H : acc.contains path) (le : EvalPaths ls ρ path (acc.eval ls ρ)) :
+    (addConst k path acc).eval ls ρ = max' (acc.eval ls ρ) (evalPath ls ρ path k) := by
+  simp [addConst]; split <;> rename_i h
+  · obtain rfl | ⟨rfl, _⟩ := h
+    · simp [evalPath]
+    · let a::path := path; let .insert h1 le h3 := le
+      have := h1 ▸ evalPath_orderedInsert (ls := ls) (ρ := ρ); simp at this
+      rw [this, Nat.max_eq_left]; simp [evalPath]; split <;> [rename_i h; simp]
+      let ⟨h1, h2⟩ := allNZ_cons.1 h; exact Nat.le_trans h1 (evalPath_le.1 le h2)
+  · refine ext_le fun x => ?_
+    rw [← Std.TreeMap.isSome_getElem?_eq_contains, Option.isSome_iff_exists] at H; let ⟨v, H⟩ := H
+    simp [eval_le, Nat.max_le, Std.TreeMap.getElem?_modify, evalPath_le, Node.eval_le, H]
+    refine ⟨fun h1 => ?_, fun ⟨h1, h2⟩ a b => ?_⟩
+    · have := h1 path; simp [Nat.max_le] at this
+      refine ⟨fun a b h3 h4 => ?_, fun h => (this h).1.1⟩
+      specialize h1 a; split at h1
+      · subst a; cases H.symm.trans h3; exact ⟨(this h4).1.2, (this h4).2⟩
+      · exact h1 _ h3 h4
+    · split
+      · subst a; rintro ⟨⟩ nz; simp [Nat.max_le, nz, h2]; exact h1 _ _ H nz
+      · exact h1 _ _
+
+theorem VarNode.addVar_le : (∀ vn ∈ VarNode.addVar v k l, vn.eval ls ρ ≤ x) ↔
+    evalParam ls ρ v + k ≤ x ∧ (∀ vn ∈ l, vn.eval ls ρ ≤ x) := by
+  simp [eval]; induction l with simp [VarNode.addVar] | cons vn l ih; split <;> simp [*]
+  · simp at *; subst v
+    rw [← and_assoc, ← Nat.max_le, Nat.add_max_add_left, Nat.max_comm, Nat.max_eq_max]
+  · rw [and_left_comm]
+
+theorem NormLevel.addNode_eval : (addNode v k path acc).eval ls ρ =
+    max' (acc.eval ls ρ) (evalPath ls ρ path (evalParam ls ρ v + k)) := by
+  refine ext_le fun x => ?_
+  simp [addNode, eval_le, Std.TreeMap.getElem?_alter, evalPath_le, Node.eval_le, Nat.max_le]
+  refine ⟨fun H => ⟨fun a b h nz => ?_, fun nz => ?_⟩, fun ⟨H1, H2⟩ a b h nz => ?_⟩
+  · have := H a; split at this
+    · subst a; simp_all [VarNode.addVar_le]
+    · exact this _ h nz
+  · have := H path; simp at this; split at this <;> specialize this _ rfl nz
+    · simp_all [VarNode.eval]
+    · simp_all [VarNode.addVar_le]
+  · split at h
+    · subst a; split at h <;> cases h
+      · simp_all [VarNode.eval]
+      · simp_all [VarNode.addVar_le]; grind
+    · grind
+
+theorem NormLevel.addVar_eval (H : acc.contains path) : (addVar v k path acc).eval ls ρ =
+    max' (acc.eval ls ρ) (evalPath ls ρ path (evalParam ls ρ v + k)) := by
+  refine ext_le fun x => ?_
+  rw [← Std.TreeMap.isSome_getElem?_eq_contains, Option.isSome_iff_exists] at H; let ⟨v, H⟩ := H
+  simp [addVar, eval_le, Nat.max_le, Std.TreeMap.getElem?_modify, evalPath_le, Node.eval_le, H]
+  refine ⟨fun H => ⟨fun a b h nz => ?_, fun nz => ?_⟩, fun ⟨H1, H2⟩ a b h nz => ?_⟩
+  · have := H a; split at this
+    · subst a; simp_all [VarNode.addVar_le]
+    · exact this _ h nz
+  · have := H path; simp at this; specialize this nz; simp_all [VarNode.addVar_le]
+  · split at h
+    · subst a; cases h; simp_all [VarNode.addVar_le]; grind
+    · grind
+
+theorem normalizeAux_eval (hu : VLevel.ofLevel ls u = some u')
+    (H : acc.contains path) (le : EvalPaths ls ρ path (acc.eval ls ρ)) :
+    (normalizeAux u path k acc).eval ls ρ =
+    max' (acc.eval ls ρ) (evalPath ls ρ path (u'.eval ρ + k)) := by
+  unfold normalizeAux; split
+  · cases hu; simp [NormLevel.addConst_eval H le, VLevel.eval]
+  · simp [VLevel.ofLevel] at hu; obtain ⟨_, hu, rfl⟩ := hu
+    simp [VLevel.eval, Nat.imax, NormLevel.addConst_eval H le]
+  · simp [VLevel.ofLevel] at hu; obtain ⟨_, hu, rfl⟩ := hu
+    rw [normalizeAux_eval hu H le, Nat.add_succ, ← Nat.succ_add]; rfl
+  · simp [VLevel.ofLevel] at hu; obtain ⟨_, hu, _, hv, rfl⟩ := hu
+    rw [normalizeAux_eval hv (normalizeAux_contains H)] <;> rw [normalizeAux_eval hu H le]
+    · rw [Nat.max_assoc, ← evalPath_max, Nat.add_max_add_right]; rfl
+    · exact le.max
+  · simp [VLevel.ofLevel] at hu; obtain ⟨_, hu, _, ⟨_, hv, rfl⟩, rfl⟩ := hu
+    rw [normalizeAux_eval hv (normalizeAux_contains H)] <;> rw [normalizeAux_eval hu H le]
+    · rw [Nat.max_assoc, Nat.add_succ, ← Nat.succ_add, ← evalPath_max, Nat.add_max_add_right]; rfl
+    · exact le.max
+  · rename_i u v w
+    simp [VLevel.ofLevel] at hu; obtain ⟨_, hu, _, ⟨_, hv, _, hw, rfl⟩, rfl⟩ := hu
+    rw [normalizeAux_eval
+        (by simpa [VLevel.ofLevel] using ⟨_, hu, _, hw, rfl⟩) (normalizeAux_contains H)] <;>
+      rw [normalizeAux_eval (by simpa [VLevel.ofLevel] using ⟨_, hu, _, hv, rfl⟩) H le]
+    · rw [Nat.max_assoc, ← evalPath_max, Nat.add_max_add_right]; simp [VLevel.eval, imax_max]
+    · exact le.max
+  · rename_i u v w
+    simp [VLevel.ofLevel] at hu; obtain ⟨_, hu, _, ⟨_, hv, _, hw, rfl⟩, rfl⟩ := hu
+    rw [normalizeAux_eval (by simpa [VLevel.ofLevel] using ⟨_, hv, _, hw, rfl⟩)
+        (normalizeAux_contains H)] <;>
+      rw [normalizeAux_eval (by simpa [VLevel.ofLevel] using ⟨_, hu, _, hw, rfl⟩) H le]
+    · rw [Nat.max_assoc, ← evalPath_max, Nat.add_max_add_right]; simp [VLevel.eval, imax_imax]
+    · exact le.max
+  · rename_i u v
+    simp [VLevel.ofLevel] at hu; obtain ⟨_, hu, _, ⟨hv, rfl⟩, rfl⟩ := hu
+    have := @evalPath_orderedInsert ls ρ v path
+    split <;> rename_i h <;> simp [h] at this
+    · rw [normalizeAux_eval hu NormLevel.addNode_contains_self] <;>
+        rw [NormLevel.addNode_eval, NormLevel.addConst_eval H le, Nat.max_assoc]
+      · rw [Nat.max_assoc, ← evalPath_max, this, evalPath_cons, ← evalPath_max,
+          Nat.add_max_add_right]; congr 2
+        simp [VLevel.eval, ← evalParam_eq hv, Nat.imax]
+        cases evalParam .. <;> simp [Nat.max_eq_max, Nat.max_comm]
+      · refine .insert h (Nat.le_trans ?_ (Nat.le_max_right ..)) le.max
+        rw [this, evalPath_cons, ← evalPath_max]; apply evalPath_mono; grind
+    · dsimp; split
+      · rw [normalizeAux_eval hu H le]
+        simp [evalPath]; split <;> [rename_i nz; simp]
+        have hm := (h ▸ mem_orderedInsert).2 (.inl rfl)
+        have ⟨p1, p2, a1, a2, a3, a4⟩ := le.of_mem hm
+        have := evalPath_le.1 a3 (allNZ_mono a1 nz)
+        simp [allNZ] at nz; specialize nz _ hm
+        simp [VLevel.eval, Nat.imax]; simp [← evalParam_eq hv]
+        revert this nz; cases evalParam .. <;> simp
+        rw [Nat.max_eq_max, Nat.max_comm (a := VLevel.eval ..), ← Nat.add_max_add_right, ← Nat.max_assoc]
+        intro h; rw [Nat.max_eq_left (b := _+1+k)]; omega
+      · rw [normalizeAux_eval hu (NormLevel.addVar_contains H)] <;> rw [NormLevel.addVar_eval H]
+        · rw [Nat.max_assoc, ← evalPath_max, Nat.add_max_add_right, this,
+            evalPath_cons, evalPath_cons]; congr 2; split <;> simp [VLevel.eval, Nat.imax]
+          rename_i h; revert h; simp [← evalParam_eq hv]
+          cases evalParam .. <;> simp [Nat.max_eq_max, Nat.max_comm]
+        · exact le.max
+  · cases hu
+  · simp [VLevel.ofLevel] at hu
+  · rename_i v; simp [VLevel.ofLevel] at hu; obtain ⟨hv, rfl⟩ := hu
+    have := @evalPath_orderedInsert ls ρ v path
+    split <;> rename_i h <;> simp [h] at this
+    · rw [NormLevel.addNode_eval, NormLevel.addConst_eval H le, Nat.max_assoc,
+        this, evalPath_cons, ← evalPath_max]
+      simp [VLevel.eval, ← evalParam_eq hv]; congr 2; split <;> simp; omega
+    · split
+      · simp [evalPath]; split <;> [rename_i nz; simp]
+        have hm := (h ▸ mem_orderedInsert).2 (.inl rfl)
+        have ⟨p1, p2, a1, a2, a3, a4⟩ := le.of_mem hm
+        have := evalPath_le.1 a3 (allNZ_mono a1 nz)
+        simp [allNZ] at nz; specialize nz _ hm
+        simp [VLevel.eval, ← evalParam_eq hv]
+        revert this nz; cases evalParam .. <;> simp; omega
+      · rw [NormLevel.addVar_eval H, this, evalPath_cons, evalPath_cons]
+        congr 2; split <;> simp [VLevel.eval, ← evalParam_eq hv]
+
+theorem NormLevel.subsumption_eval {s : NormLevel} :
+    s.subsumption.eval ls ρ = s.eval ls ρ := by
+  sorry
+
+theorem normalize_eval (hu : VLevel.ofLevel ls u = some u') :
+    (normalize u).eval ls ρ = u'.eval ρ := by
+  simp [normalize, NormLevel.subsumption_eval]
+  exact normalizeAux_eval hu (by simp) .nil
+
+theorem Node.eval_congr {a b : Node} (H : a == b) : a.eval ls ρ = b.eval ls ρ := by
+  simp [instBEqNode] at H; simp [H, eval]
+
+theorem NormLevel.eval_congr {a b : NormLevel} (H : a == b) : a.eval ls ρ = b.eval ls ρ := by
+  simp only [instBEqNormLevel, Std.TreeMap.all_eq_all_toList,
+    Bool.and_eq_true, List.all_eq_true] at H
+  suffices ∀ {a b : NormLevel}, (∀ x ∈ a.toList, b.get? x.1 == some x.2) →
+      a.eval ls ρ ≤ b.eval ls ρ from Nat.le_antisymm (this H.1) (this H.2)
+  clear a b H; intro a b H
+  simp only [eval, Std.TreeMap.foldl_eq_foldl_toList]
+  rw [← a.toList.reverse_reverse] at H ⊢; generalize a.toList.reverse = a at H ⊢
+  simp only [List.mem_reverse, Std.TreeMap.get?_eq_getElem?, List.foldl_reverse] at H ⊢
+  induction a with | nil => exact Nat.zero_le _ | cons p l ih; let (x, y) := p
+  simp only [List.mem_cons, or_imp, forall_and, forall_eq, List.foldr_cons] at H ⊢
+  refine Nat.max_le.2 ⟨ih H.2, ?_⟩
+  let ⟨y', h1, h2⟩ := Option.beq_some_iff.1 H.1
+  have H := Std.TreeMap.mem_toList_iff_getElem?_eq_some.2 h1
+  rw [← b.toList.reverse_reverse] at H ⊢; generalize b.toList.reverse = b at H ⊢
+  simp only [List.mem_reverse, List.foldl_reverse] at H ⊢
+  induction b with | nil => cases H | cons p l ih; let (x, y) := p
+  simp; obtain ⟨⟩ | ⟨_, (H : _ ∈ l)⟩ := H
+  · exact Node.eval_congr h2 ▸ Nat.le_max_right ..
+  · exact Nat.le_trans (ih H) (Nat.le_max_left ..)
+
+end Normalize
+
 theorem isEquiv'_wf (h : isEquiv' u v)
-    (hu : VLevel.ofLevel ls u = some u') (hv : VLevel.ofLevel ls v = some v') : u' ≈ v' := sorry
+    (hu : VLevel.ofLevel ls u = some u') (hv : VLevel.ofLevel ls v = some v') : u' ≈ v' := by
+  simp [isEquiv'] at h; obtain rfl | h := h
+  · cases hu.symm.trans hv; rfl
+  refine VLevel.equiv_def.2 fun ls' => ?_
+  rw [← Normalize.normalize_eval hu, ← Normalize.normalize_eval hv]
+  exact Normalize.NormLevel.eval_congr h
 
 theorem isEquivList_wf (H : Level.isEquivList us vs) :
     List.mapM (VLevel.ofLevel Us) us = some us' →
